theories/L/Complexity/Cook/SharedSAT.v
@@ -1,0 +1,13 @@
+From Undecidability.L Require Import L.
+From Undecidability.L.Datatypes Require Import LLists. 
+Require Import Lia. 
+
+Notation var := (nat) (only parsing). 
+Notation assgn := (list var). 
+
+Definition evalVar a v  := list_in_decb Nat.eqb a v.
+
+Lemma evalVar_in_iff a v : evalVar a v = true <-> v el a. 
+Proof. 
+  unfold evalVar. rewrite list_in_decb_iff; [easy | symmetry; apply Nat.eqb_eq].
+Qed.
